theories/simulations/lsim/LSimTactics.v
@@ -13,9 +13,24 @@ Ltac ired_t := try (prw _red_gen 1 1 0).
 Ltac ired_both := ired_s; ired_t.
 
 Ltac prep := ired_both. (* prepare *)
-  
+
+Ltac apply_lsimC_spec :=
+  match goal with
+  | [ |- gpaco8 (_lsim ?fl_src ?fl_tgt ?lw ?my_tid)
+          _ _ _ _ _ _ _ _ _ _ _ ] =>
+    apply (lsimC_spec fl_src fl_tgt lw my_tid)
+  end.
+
+Ltac guclo_lflagC :=
+  match goal with
+  | [ |- gpaco8 (_lsim ?fl_src ?fl_tgt ?lw ?my_tid)
+          _ _ _ _ _ _ _ _ _ _ _ ] =>
+    guclo (lflagC_spec fl_src fl_tgt lw my_tid);
+      try exact (lsim_mon fl_src fl_tgt lw my_tid)
+  end.
+
 Ltac _step :=
-  ired_both; apply lsimC_spec; econs; i;
+  ired_both; apply_lsimC_spec; econs; i;
   match goal with
   | [ |- exists (_ : unit), _ ] => esplits; [eauto|..]; i
   | [ |- exists _, _ ] => fail 1
